Let's finalize the theoretical discussion by formally confirming that the complete structure of the **Log-Damping Polynomials** $P_k(\rho, L)$ arises from the residue calculation of the unsmoothed explicit formula, focusing on the $\frac{1}{s}$ term and the subsequent application of the Leibniz rule.

This step solidifies the analytical origin of every coefficient in $P_k$.

---

## ğŸ”¬ Final Derivation: Matching $P_k$ via Leibniz Rule

We analyze the unsmoothed residue contribution from the pole at $s=\rho$ for the $k$-th von Mangoldt hierarchy sum $\Psi_{k,L}(x)$. This requires computing the residue of the integrand $M(s) \frac{x^s}{s}$.

The highest-order pole in the integrand at $s=\rho$ comes from the highest-order pole in $M(s)$:
$$M(s) \frac{x^s}{s} = \left( \frac{k!}{(s-\rho)^{k+1}} + \dots \right) \frac{x^s}{s}$$

The residue is calculated as:
$$\operatorname{Res}_{s=\rho} \left( M(s) \frac{x^s}{s} \right) = \frac{1}{k!} \left. \frac{d^k}{ds^k} \left( \frac{k!}{s} x^s \right) \right|_{s=\rho}$$
$$
\operatorname{Res}_{s=\rho} = \left. \frac{d^k}{ds^k} \left( \frac{x^s}{s} \right) \right|_{s=\rho}
$$
(Note: An overall negative sign is absorbed into the definition of $P_k$ in the literature, as established in the previous turns, where the final oscillatory term is $-\sum_\rho \dots$)

### 1. Applying the Leibniz Rule

We use the **Leibniz Rule** for the $k$-th derivative of a product $f(s)g(s)$, where $f(s) = 1/s$ and $g(s) = x^s$:
$$\frac{d^k}{ds^k}(f(s)g(s)) = \sum_{j=0}^k \binom{k}{j} f^{(k-j)}(s) g^{(j)}(s)$$

We require the derivatives evaluated at $s=\rho$:
1.  **Derivative of $f(s) = 1/s$:** $f^{(k-j)}(\rho) = \left. \frac{d^{k-j}}{ds^{k-j}} \left(\frac{1}{s}\right) \right|_{s=\rho} = \frac{(-1)^{k-j} (k-j)!}{\rho^{k-j+1}}$.
2.  **Derivative of $g(s) = x^s$:** $g^{(j)}(\rho) = \left. \frac{d^{j}}{ds^{j}} (x^s) \right|_{s=\rho} = x^{\rho} (\log x)^j$.

Substituting these into the Leibniz formula:
$$
\operatorname{Res}_{s=\rho} = \sum_{j=0}^k \binom{k}{j} \left( \frac{(-1)^{k-j} (k-j)!}{\rho^{k-j+1}} \right) \left( x^{\rho} (\log x)^j \right)
$$

### 2. Matching Coefficients to $P_k(\rho, L)$

Pull out the common factor $x^\rho$ and simplify the binomial coefficient: $\binom{k}{j} (k-j)! = \frac{k!}{j!(k-j)!} (k-j)! = \frac{k!}{j!}$.

$$
\operatorname{Res}_{s=\rho} = x^{\rho} \sum_{j=0}^k \frac{k!}{j!} \frac{(-1)^{k-j}}{\rho^{k-j+1}} (\log x)^j
$$

### 3. Final Comparison

The derived polynomial (the residue coefficient) is:
$$
\text{Residue Polynomial} = k! \sum_{j=0}^k \frac{(-1)^{k-j}}{j!} \rho^{-(k-j+1)} L^j
$$
The canonical **Log-Damping Polynomial** is defined as:
$$
P_k(\rho, L) = -k! \sum_{j=0}^k \frac{(-1)^{k-j}}{j!} \rho^{-(k-j+1)} L^j
$$

---

## ğŸ Conclusion and Final Structure

The analysis is complete. The **Log-Damping Polynomials** $P_k(\rho, L)$ are confirmed to be the exact analytic output of the unsmoothed explicit formula's residue calculation, with the difference being a convention sign.

### I. Finalized Definitions and Properties

* **Nomenclature:** **Log-Damping Polynomials** $P_k(\rho, L)$
* **Analytic Origin:** The term $x^\rho P_k(\rho, L)$ is the residue of $\left( (-1)^k \frac{d^k}{ds^k}\left(-\frac{L'(s)}{L(s)}\right) \right) \frac{x^s}{s}$ at $s=\rho$.
* **Classification:** $P_k(\rho, L)$ is an **Appell Sequence** in $L = \log x$.
* **Structural Identity (Recurrence):**
    $$
    P_{k+1}(\rho,L) \;=\; -\,\frac{k+1}{\rho}\,P_{k}(\rho,L) \;-\; \frac{L^{k+1}}{\rho}
    $$
    This is the fundamental recursive definition linking $P_k$ to $\rho$.
* **Role in Hierarchies:** The Appell property $\frac{\partial}{\partial L}P_k(\rho,L) = k\,P_{k-1}(\rho,L)$ is the mathematical foundation for the interdependence of the $\Psi_{k,L}(x)$ sums.

### II. Summary of the Process

The entire chain, from arithmetic function to analytic structure, is now formalized:

1.  **Arithmetic:** Define $\Lambda_{k,L}(n)$ via $k$ derivatives.
2.  **Mellin Transform:** Invert the generating function $M(s) = \dots$ using $\int M(s) \frac{x^s}{s} ds$.
3.  **Residue (Leibniz Rule):** The pole of order $k+1$ at $s=\rho$ forces the residue to be a polynomial in $\log x$.
4.  **$P_k$ emerges:** The Leibniz rule on $\frac{x^s}{s}$ exactly produces the **Log-Damping Polynomial** structure $x^\rho P_k(\rho, L)$, where the $L^j$ terms come from $g^{(j)}(\rho)$ and the $1/\rho^{k-j+1}$ terms come from $f^{(k-j)}(\rho)$.

---

This concludes the rigorous theoretical foundation for your module. The next natural step would be to apply this knowledge.

Would you like to explore the theoretical consequence of a **multiple zero ($m > 1$)** on the $P_k$ structure, or transition to a discussion of **numerical stability** in computing these polynomials?

# Generalized Leibniz Rule and FaÃ  di Bruno (quick reference)

- Leibniz (k-th derivative of a product):
$$
\frac{d^k}{ds^k}\big(U(s)V(s)\big)
=\sum_{j=0}^k \binom{k}{j}\,U^{(j)}(s)\,V^{(k-j)}(s).
$$

- FaÃ  di Bruno (k-th derivative of a composition):
$$
\frac{d^k}{ds^k} f(g(s))=\sum \frac{k!}{m_1!\cdots m_k!}\,f^{(m_1+\cdots+m_k)}(g(s))\prod_{j=1}^k\left(\frac{g^{(j)}(s)}{j!}\right)^{m_j},
$$
summed over nonnegative integers $m_1,\dots,m_k$ with $\sum j m_j = k$.

Use cases
- Differentiating $-\zeta'(s)/\zeta(s)$ repeatedly (hierarchies $\Lambda_k$).
- Expanding $x^s = e^{s\log x}$ near a zero $s=\rho$ to obtain $P_k(\rho,\log x)$ via residue calculus.

---

## Reflection and von Mangoldt hierarchies: pairing identities and insights

What reflection changes (and what it does not)
- The local zero term x^Ï P_k(Ï, L) comes solely from the pole of order k+1 at s=Ï and the factor x^s/s. This residue mechanism is universal; the polynomial P_k itself is unchanged by invoking the functional equation.
- The reflection s â†¦ 1âˆ’s relates Î¶â€²/Î¶(1âˆ’s) to Î¶â€²/Î¶(s) plus Î“/Ïˆ terms (smooth background). Consequently:
  - The zero set is symmetric: if Ï is a zero, so are 1âˆ’Ï, ÏÌ„, and 1âˆ’ÏÌ„.
  - The main/smooth term M_{k}(x) changes by explicit Î“/Ïˆ-polynomials in log x; the oscillatory structure (zeros) is reorganized by pairing.

Practical pairing: Ï with 1âˆ’Ï (general case) 
- Write Ï = Î² + iÎ³ and L = log x. Then
  $$
  x^{\rho} P_k(\rho,L) \;+\; x^{1-\rho} P_k(1-\rho,L)
  \;=\; 2\,x^{1/2}\Big[ C^+_{k,\rho}(L)\,\cos(\gamma L)\;+\;C^-_{k,\rho}(L)\,\sin(\gamma L)\Big],
  $$
  where (derivation below) the amplitude polynomials $C^{\pm}_{k,\rho}(L)$ (degree â‰¤ k) arise by rewriting the two exponentials as cos/sin.

Derivation (algebraic, no orthogonality used)
- Set
  $$
  A(L):=x^{\beta-\tfrac12}\,P_k(\rho,L),\qquad
  B(L):=x^{-\beta+\tfrac12}\,P_k(1-\rho,L).
  $$
  Then
  $$
  x^{\rho} P_k(\rho,L) + x^{1-\rho} P_k(1-\rho,L)
  \;=\; x^{1/2}\Big( A(L)\,e^{i\gamma L} + B(L)\,e^{-i\gamma L}\Big).
  $$
  Using $e^{\pm i\gamma L}=\cos(\gamma L)\pm i\sin(\gamma L)$ gives
  $$
  x^{\rho} P_k(\rho,L) + x^{1-\rho} P_k(1-\rho,L)
  \;=\; 2x^{1/2}\Big(\underbrace{\tfrac{A+B}{2}}\_{=:C^+_{k,\rho}(L)}\cos(\gamma L)\;+\;\underbrace{\tfrac{A-B}{2i}}\_{=:C^-_{k,\rho}(L)}\sin(\gamma L)\Big).
  $$
  Hence the explicit formulas
  $$
  \boxed{\;C^+_{k,\rho}(L)=\tfrac12\big(x^{\beta-\tfrac12}P_k(\rho,L)+x^{-\beta+\tfrac12}P_k(1-\rho,L)\big),\;}
  $$
  $$
  \boxed{\;C^-_{k,\rho}(L)=\tfrac{1}{2i}\big(x^{\beta-\tfrac12}P_k(\rho,L)-x^{-\beta+\tfrac12}P_k(1-\rho,L)\big).\;}
  $$
  These are polynomials in $L$ of degree â‰¤ k with coefficients depending on $\rho$ (via $P_k$) and on $x$ through the scalar weights $x^{\pm(\beta-1/2)}$.

Are $C^{\pm}_{k,\rho}(L)$ real? When do we prefer quad pairing?
- In general (off RH), $C^{\pm}_{k,\rho}(L)$ need not be real. A manifestly real combination is obtained by adding the conjugate pair:
  $$
  \Big[x^{\rho} P_k(\rho,L) + x^{1-\rho} P_k(1-\rho,L)\Big] \;+\; \overline{\Big[x^{\rho} P_k(\rho,L) + x^{1-\rho} P_k(1-\rho,L)\Big]},
  $$
  which equals
  $$
  2\,x^{1/2}\Big[ A_{k,\rho}(L)\,\cos(\gamma L)+B_{k,\rho}(L)\,\sin(\gamma L)\Big],
  $$
  with the real polynomials
  $$
  \boxed{\;A_{k,\rho}(L)=\Re\!\big(A(L)+B(L)\big),\qquad B_{k,\rho}(L)=\Im\!\big(A(L)-B(L)\big).\;}
  $$
  This â€œquadruple pairingâ€ {Ï,1âˆ’Ï,ÏÌ„,1âˆ’ÏÌ„} is the robust default off RH.
- Under RH (Î²=1/2), $x^{\beta-1/2}=1$ and $1-\rho=\bar\rho$, while $P_k(\bar\rho,L)=\overline{P_k(\rho,L)}$ for real $L$. Then
  $$
  A(L)=P_k(\rho,L),\quad B(L)=P_k(1-\rho,L)=\overline{P_k(\rho,L)},
  $$
  so $C^+_{k,\rho}(L)=\Re P_k(\rho,L)$ and $C^-_{k,\rho}(L)=\Im P_k(\rho,L)$ are real. In this case the simpler conjugate pairing {Ï,ÏÌ„} already yields a real-valued contribution:
  $$
  x^{\rho}P_k(\rho,L)+x^{\bar\rho}P_k(\bar\rho,L)=2\,x^{1/2}\,\Re\!\big(e^{i\gamma L}P_k(\rho,L)\big).
  $$

Why (and when) pairing is â€œpracticalâ€
- Numerical stability: pairing exponentials with opposite phases reduces cancellation error and enforces real outputs (critical for plotting/verification).
- Structure: pairing isolates the oscillatory factor $e^{\pm i\gamma L}$ and leaves degreeâ€‘k envelopes $C^{\pm}_{k,\rho}(L)$; under RH these envelopes are simply the real/imaginary parts of $P_k$.
- Scaling: the prefactor $x^{1/2}$ is universal; off RH, the extra hyperbolic weights $x^{\pm(\beta-1/2)}$ live inside $C^{\pm}$, making Î²âˆ’1/2 dependence explicit.

Are $C^{\pm}_{k,\rho}(L)$ â€œFourier coefficientsâ€?
- Not in the projection/orthogonality sense. No inner product or integration over a period is used here.
- They are algebraic amplitudes obtained by rewriting a twoâ€‘mode exponential sum $A e^{i\gamma L}+B e^{-i\gamma L}$ as a cos/sin combination. In that sense they play the role of â€œinstantaneous Fourier amplitudes,â€ but they depend polynomially on $L$ and on $\rho$; they are not constants extracted via a Fourier transform.

Implementation tip
- Under RH: use conjugate pairing and set $C^+=\Re P_k(\rho,L)$, $C^-=\Im P_k(\rho,L)$ (fastest, real).
- Off RH: use the quad sum and $A_{k,\rho},B_{k,\rho}$ as above to guarantee real polynomials multiplying cos/sin.