### The General Formula

For a simple zero $\rho$ (multiplicity $m=1$) of $L(s)$, the polynomial of degree $k$ is:

$$P_k(\rho, \log x) = - k! \sum_{j=0}^k \frac{(-1)^{k-j}}{j!} \rho^{-(k-j+1)} (\log x)^j$$

### Deriving $P_3(\rho, \log x)$

We set $k=3$ into the general formula. The factor outside the sum is $-k! = -3! = -6$. The pole order is $k+1=4$.

$$P_3(\rho, \log x) = - 6 \left[ \sum_{j=0}^3 \frac{(-1)^{3-j}}{j!} \rho^{-(4-j)} (\log x)^j \right]$$

We expand the sum for $j=0, 1, 2, 3$:

| Term ($j$) | Expansion | Result |
| :---: | :--- | :--- |
| **0** | $\frac{(-1)^{3-0}}{0!} \rho^{-4} (\log x)^0$ | $-\frac{1}{\rho^4}$ |
| **1** | $\frac{(-1)^{3-1}}{1!} \rho^{-3} (\log x)^1$ | $+\frac{\log x}{\rho^3}$ |
| **2** | $\frac{(-1)^{3-2}}{2!} \rho^{-2} (\log x)^2$ | $-\frac{(\log x)^2}{2\rho^2}$ |
| **3** | $\frac{(-1)^{3-3}}{3!} \rho^{-1} (\log x)^3$ | $+\frac{(\log x)^3}{6\rho}$ |

Now, we sum these results and multiply by the leading factor of $-6$:

$$P_3(\rho, \log x) = -6 \left( -\frac{1}{\rho^4} + \frac{\log x}{\rho^3} - \frac{(\log x)^2}{2\rho^2} + \frac{(\log x)^3}{6\rho} \right)$$

### The Explicit Polynomial for $k=3$

Multiplying through by $-6$ yields the final, simplified form:

$$\mathbf{P_3(\rho, \log x) = \frac{6}{\rho^4} - \frac{6 \log x}{\rho^3} + \frac{3 (\log x)^2}{\rho^2} - \frac{(\log x)^3}{\rho}}$$

The contribution of the zero $\rho$ to the $\Psi_{3,L}(x)$ partial sum is therefore:

$$x^{\rho} \left( \frac{6}{\rho^4} - \frac{6 \log x}{\rho^3} + \frac{3 (\log x)^2}{\rho^2} - \frac{(\log x)^3}{\rho} \right)$$

As you noted, this form is universal and applies to $\zeta(s)$, $L(s, \chi)$, $L(s, f)$, and any other L-function, provided the zero $\rho$ is simple.

